coq/Translation/LambdaNRAtoNRAEnv.v
@@ -47,146 +47,191 @@ Section LambdaNRAtoNRAEnv.
     end.
 
   Context (h:brand_relation_t).
-  Context (global_env:bindings).
 
-  Lemma lambda_nra_to_nraenv_never_uses_id :
-    forall env:bindings, forall q:lambda_nra, forall d1 d2:data,
-          nraenv_eval h global_env
-                      (lambda_nra_to_nraenv q) (drec env) d1 =
-          nraenv_eval h global_env
-                      (lambda_nra_to_nraenv q) (drec env) d2.
-  Proof.
-    lambda_nra_cases (induction q) Case
-    ; intros; unfold nraenv_eval in *; simpl in *
-    ; autorewrite with lambda_nra; try reflexivity.
-    - Case "LNRABinop"%string.
-      rewrite (IHq1 d1 d2).
-      rewrite (IHq2 d1 d2).
-      reflexivity.
-    - Case "LNRAUnop"%string.
-      rewrite (IHq d1 d2).
-      reflexivity.
-    - Case "LNRAMap"%string.
-      rewrite (IHq2 d1 d2).
-      reflexivity.
-    - Case "LNRAMapConcat"%string.
-      rewrite (IHq2 d1 d2).
-      reflexivity.
-    - Case "LNRAProduct"%string.
-      rewrite (IHq1 d1 d2).
-      rewrite (IHq2 d1 d2).
-      reflexivity.
-    - Case "LNRAFilter"%string.
-      rewrite (IHq2 d1 d2).
-      reflexivity.
-  Qed.
+  Section Translation.
+    Context (global_env:bindings).
 
-  Theorem lambda_nra_to_nraenv_correct :
-    forall q:lambda_nra, forall env:bindings, forall d:data,
-      lambda_nra_eval h global_env env q =
-      nraenv_eval h global_env
-                  (lambda_nra_to_nraenv q) (drec env) d.
-  Proof.
-    lambda_nra_cases (induction q) Case
-    ; intros; unfold nraenv_eval in *; simpl in *
-    ; autorewrite with lambda_nra; try reflexivity.
-    - Case "LNRABinop"%string.
-      rewrite (IHq1 _ d).
-      rewrite (IHq2 _ d).
-      reflexivity.
-    - Case "LNRAUnop"%string.
-      rewrite (IHq _ d).
-      reflexivity.
-    - Case "LNRAMap"%string.
-      rewrite <- (IHq2 _ d).
-      simpl.
-      apply olift_ext; intros.
-      apply lift_oncoll_ext; intros.
-      subst.
-      f_equal.
-      apply rmap_ext; intros.
-      autorewrite with lambda_nra.
-      rewrite (IHq1 _ x).
-      admit.
-    - Case "LNRAMapConcat"%string.
-      admit.
-    - Case "LNRAProduct"%string.
-      admit.
-    - Case "LNRAFilter"%string.
-      admit.
-  Admitted.
+    Lemma lambda_nra_to_nraenv_never_uses_id :
+      forall env:bindings, forall q:lambda_nra, forall d1 d2:data,
+            nraenv_eval h global_env
+                        (lambda_nra_to_nraenv q) (drec env) d1 =
+            nraenv_eval h global_env
+                        (lambda_nra_to_nraenv q) (drec env) d2.
+    Proof.
+      lambda_nra_cases (induction q) Case
+      ; intros; unfold nraenv_eval in *; simpl in *
+      ; autorewrite with lambda_nra; try reflexivity.
+      - Case "LNRABinop"%string.
+        rewrite (IHq1 d1 d2).
+        rewrite (IHq2 d1 d2).
+        reflexivity.
+      - Case "LNRAUnop"%string.
+        rewrite (IHq d1 d2).
+        reflexivity.
+      - Case "LNRAMap"%string.
+        rewrite (IHq2 d1 d2).
+        reflexivity.
+      - Case "LNRAMapConcat"%string.
+        rewrite (IHq2 d1 d2).
+        reflexivity.
+      - Case "LNRAProduct"%string.
+        rewrite (IHq1 d1 d2).
+        rewrite (IHq2 d1 d2).
+        reflexivity.
+      - Case "LNRAFilter"%string.
+        rewrite (IHq2 d1 d2).
+        reflexivity.
+    Qed.
+
+    (** Evaluation for lambda nra is the same as evaluation for translated expression to NRAEnv
+      - Note that only the global and local environments matter.
+        The 'input value' for NRA (d in the theorem) is not used on the LambdaNRA side.
+        This is consistent with the previous theorem showing that any 'd' does not matter.
+     *)
+    Theorem lambda_nra_to_nraenv_correct :
+      forall q:lambda_nra, forall env:bindings, forall d:data,
+            lambda_nra_eval h global_env env q =
+            nraenv_eval h global_env
+                        (lambda_nra_to_nraenv q) (drec env) d.
+    Proof.
+      lambda_nra_cases (induction q) Case
+      ; intros; unfold nraenv_eval in *; simpl in *
+      ; autorewrite with lambda_nra; try reflexivity.
+      - Case "LNRABinop"%string.
+        rewrite (IHq1 _ d).
+        rewrite (IHq2 _ d).
+        reflexivity.
+      - Case "LNRAUnop"%string.
+        rewrite (IHq _ d).
+        reflexivity.
+      - Case "LNRAMap"%string.
+        rewrite <- (IHq2 _ d).
+        simpl.
+        apply olift_ext; intros.
+        apply lift_oncoll_ext; intros.
+        subst.
+        f_equal.
+        apply rmap_ext; intros.
+        autorewrite with lambda_nra.
+        rewrite (IHq1 _ x).
+        reflexivity.
+      - Case "LNRAMapConcat"%string.
+        rewrite <- (IHq2 _ d).
+        apply olift_ext; intros.
+        apply lift_oncoll_ext; intros.
+        subst.
+        f_equal.
+        apply rmap_concat_ext; intros.
+        autorewrite with lambda_nra.
+        rewrite (IHq1 _ x).
+        reflexivity.
+      - Case "LNRAProduct"%string.
+        rewrite (IHq1 _ d).
+        rewrite (IHq2 _ d).
+        reflexivity.
+      - Case "LNRAFilter"%string.
+        rewrite <- (IHq2 _ d).
+        apply olift_ext; intros.
+        apply lift_oncoll_ext; intros.
+        subst.
+        f_equal.
+        apply lift_filter_ext; intros.
+        autorewrite with lambda_nra.
+        rewrite (IHq1 _ x).
+        reflexivity.
+    Qed.
   
-  Theorem nraenv_of_lnra_lambda_correct :
-    forall env:bindings, forall lop:lnra_lambda, forall d:data,
-      lnra_lambda_eval h global_env env lop d =
-      nraenv_eval h global_env
-                  (nraenv_of_lnra_lambda lop) (drec env) d.
-  Proof.
-    destruct lop.
-    revert env s.
-    lambda_nra_cases (induction l) Case
-    ; intros; unfold nraenv_eval in *; simpl in *
-    ; autorewrite with lambda_nra.
-    - Case "LNRAVar"%string.
-      unfold edot, rec_concat_sort.
-      rewrite assoc_lookupr_drec_sort.
-      trivial.
-    - Case "LNRATable"%string.
-      unfold edot, rec_concat_sort.
-      trivial.
-    - Case "LNRAConst"%string.
-      trivial.
-    - Case "LNRABinop"%string.
-      rewrite <- IHl1, <- IHl2.
-      trivial.
-    - Case "LNRAUnop"%string.
-      rewrite <- IHl.
-      trivial.
-    - Case "LNRAMap"%string.
-      rewrite <- IHl2.
-      apply olift_ext; intros.
-      apply lift_oncoll_ext; intros.
-      subst.
-      f_equal.
-      apply rmap_ext; intros.
-      rewrite IHl1.
-      rewrite rec_sort_rec_sort_app1.
-      trivial.
-    - Case "LNRAMapConcat"%string.
-      rewrite <- IHl2.
-      apply olift_ext; intros.
-      apply lift_oncoll_ext; intros.
-      subst.
-      f_equal.
-      apply rmap_concat_ext; intros.
-      rewrite IHl1.
-      rewrite rec_sort_rec_sort_app1.
-      trivial.
-    - Case "LNRAProduct"%string.
-      rewrite <- IHl1, <- IHl2.
-      trivial.
-    - Case "LNRAFilter"%string.
-      rewrite <- IHl2.
-      apply olift_ext; intros.
-      apply lift_oncoll_ext; intros.
-      subst.
-      f_equal.
-      apply lift_filter_ext; intros.
-      rewrite IHl1.
-      rewrite rec_sort_rec_sort_app1.
-      trivial.
-  Qed.
+    Theorem nraenv_of_lnra_lambda_correct :
+      forall env:bindings, forall lop:lnra_lambda, forall d:data,
+            lnra_lambda_eval h global_env env lop d =
+            nraenv_eval h global_env
+                        (nraenv_of_lnra_lambda lop) (drec env) d.
+    Proof.
+      destruct lop.
+      revert env s.
+      lambda_nra_cases (induction l) Case
+      ; intros; unfold nraenv_eval in *; simpl in *
+      ; autorewrite with lambda_nra.
+      - Case "LNRAVar"%string.
+        unfold edot, rec_concat_sort.
+        rewrite assoc_lookupr_drec_sort.
+        trivial.
+      - Case "LNRATable"%string.
+        unfold edot, rec_concat_sort.
+        trivial.
+      - Case "LNRAConst"%string.
+        trivial.
+      - Case "LNRABinop"%string.
+        rewrite <- IHl1, <- IHl2.
+        trivial.
+      - Case "LNRAUnop"%string.
+        rewrite <- IHl.
+        trivial.
+      - Case "LNRAMap"%string.
+        rewrite <- IHl2.
+        apply olift_ext; intros.
+        apply lift_oncoll_ext; intros.
+        subst.
+        f_equal.
+        apply rmap_ext; intros.
+        rewrite IHl1.
+        rewrite rec_sort_rec_sort_app1.
+        trivial.
+      - Case "LNRAMapConcat"%string.
+        rewrite <- IHl2.
+        apply olift_ext; intros.
+        apply lift_oncoll_ext; intros.
+        subst.
+        f_equal.
+        apply rmap_concat_ext; intros.
+        rewrite IHl1.
+        rewrite rec_sort_rec_sort_app1.
+        trivial.
+      - Case "LNRAProduct"%string.
+        rewrite <- IHl1, <- IHl2.
+        trivial.
+      - Case "LNRAFilter"%string.
+        rewrite <- IHl2.
+        apply olift_ext; intros.
+        apply lift_oncoll_ext; intros.
+        subst.
+        f_equal.
+        apply lift_filter_ext; intros.
+        rewrite IHl1.
+        rewrite rec_sort_rec_sort_app1.
+        trivial.
+    Qed.
 
-  Definition eval_nraenv_q (Qe:nraenv) (input:data) : option data :=
-    nraenv_eval h global_env Qe (drec nil) input.
+    Definition eval_nraenv_q (Qe:nraenv) (input:data) : option data :=
+      nraenv_eval h global_env Qe (drec nil) input.
 
-  Theorem eval_nraenv_q_correct (Q:lambda_nra -> lambda_nra) (input:data) :
-    eval_lnra_lambda h global_env Q input = eval_nraenv_q (nraenv_of_lnra_lambda (q_to_lambda Q)) input.
-  Proof.
-    unfold eval_lnra_lambda, eval_nraenv_q.
-    rewrite nraenv_of_lnra_lambda_correct.
-    reflexivity.
-  Qed.
+    Theorem eval_nraenv_q_correct (Q:lambda_nra -> lambda_nra) (input:data) :
+      lnra_lambda_eval_top h Q global_env input = eval_nraenv_q (nraenv_of_lnra_lambda (q_to_lambda Q)) input.
+    Proof.
+      unfold lnra_lambda_eval_top, eval_nraenv_q.
+      rewrite nraenv_of_lnra_lambda_correct.
+      reflexivity.
+    Qed.
+  End Translation.
+
+  Section Top.
+    Definition lambda_nra_to_nraenv_top (q:lambda_nra) : nraenv :=
+      lambda_nra_to_nraenv q.
+
+    Theorem lambda_nra_to_nraenv_top_correct :
+      forall q:lambda_nra, forall global_env:bindings,
+          lambda_nra_eval_top h q global_env =
+          nraenv_eval_top h (lambda_nra_to_nraenv_top q) global_env.
+    Proof.
+      intros.
+      unfold lambda_nra_to_nraenv_top.
+      unfold lambda_nra_eval_top.
+      unfold nraenv_eval_top.
+      rewrite (lambda_nra_to_nraenv_correct (rec_sort global_env) q nil dunit).
+      reflexivity.
+    Qed.
+      
+  End Top.
 
 End LambdaNRAtoNRAEnv.
 
